theories/logrel/F_mu_ref_conc/binary/rules.v
@@ -2,7 +2,7 @@ From iris.algebra Require Import excl auth frac agree gmap list.
 From iris.proofmode Require Import tactics.
 From iris.program_logic Require Export language ectx_language ectxi_language.
 From iris.program_logic Require Import lifting.
-From iris_examples.logrel.F_mu_ref_conc Require Export rules.
+From iris_examples.logrel.F_mu_ref_conc Require Export wp_rules.
 Import uPred.
 
 Definition specN := nroot .@ "spec".
@@ -181,7 +181,8 @@ Section cfg.
     rewrite /heapS_mapsto own_valid !discrete_valid auth_frag_valid.
     by apply pure_mono=> -[_] /singleton_valid [??].
   Qed.
-  Lemma mapstoS_valid_2 l q1 q2 v1 v2 : l ↦ₛ{q1} v1 -∗ l ↦ₛ{q2} v2 -∗ ✓ (q1 + q2)%Qp.
+  Lemma mapstoS_valid_2 l q1 q2 v1 v2 :
+    l ↦ₛ{q1} v1 -∗ l ↦ₛ{q2} v2 -∗ ✓ (q1 + q2)%Qp.
   Proof.
     iIntros "H1 H2". iDestruct (mapstoS_combine with "H1 H2") as "[? ->]".
     by iApply (mapstoS_valid l _ v2).
@@ -226,7 +227,8 @@ Section cfg.
     iInv specN as (tp σ) ">[Hown Hrtc]" "Hclose".
     iDestruct "Hrtc" as %Hrtc.
     iDestruct (own_valid_2 with "Hown Hj")
-      as %[[Htpj%tpool_singleton_included' _]%prod_included ?]%auth_both_valid_discrete.
+      as %[[Htpj%tpool_singleton_included' _]%prod_included ?]
+          %auth_both_valid_discrete.
     iMod (own_update_2 with "Hown Hj") as "[Hown Hj]".
     { by eapply auth_update, prod_local_update_1,
         singleton_local_update, (exclusive_local_update _ (Excl (fill K e'))). }
@@ -274,7 +276,8 @@ Section cfg.
     iInv specN as (tp σ) ">[Hown %]" "Hclose".
     destruct (exist_fresh (dom (gset positive) σ)) as [l Hl%not_elem_of_dom].
     iDestruct (own_valid_2 with "Hown Hj")
-      as %[[?%tpool_singleton_included' _]%prod_included ?]%auth_both_valid_discrete.
+      as %[[?%tpool_singleton_included' _]%prod_included ?]
+          %auth_both_valid_discrete.
     iMod (own_update_2 with "Hown Hj") as "[Hown Hj]".
     { by eapply auth_update, prod_local_update_1,
         singleton_local_update, (exclusive_local_update _ (Excl (fill K (Loc l)))). }
@@ -318,9 +321,11 @@ Section cfg.
     rewrite /spec_ctx /tpool_mapsto /heapS_mapsto.
     iInv specN as (tp σ) ">[Hown %]" "Hclose".
     iDestruct (own_valid_2 with "Hown Hj")
-      as %[[?%tpool_singleton_included' _]%prod_included _]%auth_both_valid_discrete.
+      as %[[?%tpool_singleton_included' _]
+             %prod_included _]%auth_both_valid_discrete.
     iDestruct (own_valid_2 with "Hown Hl")
-      as %[[_ Hl%heap_singleton_included]%prod_included _]%auth_both_valid_discrete.
+      as %[[_ Hl%heap_singleton_included]%prod_included _]
+          %auth_both_valid_discrete.
     iMod (own_update_2 with "Hown Hj") as "[Hown Hj]".
     { by eapply auth_update, prod_local_update_1, singleton_local_update,
         (exclusive_local_update _ (Excl (fill K Unit))). }
@@ -343,7 +348,8 @@ Section cfg.
     rewrite /spec_ctx /tpool_mapsto /heapS_mapsto.
     iInv specN as (tp σ) ">[Hown %]" "Hclose".
     iDestruct (own_valid_2 with "Hown Hj")
-      as %[[?%tpool_singleton_included' _]%prod_included ?]%auth_both_valid_discrete.
+      as %[[?%tpool_singleton_included' _]%prod_included ?]
+          %auth_both_valid_discrete.
     iDestruct (own_valid_2 with "Hown Hl")
       as %[[_ ?%heap_singleton_included]%prod_included _]%auth_both_valid_discrete.
     iMod (own_update_2 with "Hown Hj") as "[Hown Hj]".
@@ -364,9 +370,11 @@ Section cfg.
     rewrite /spec_ctx /tpool_mapsto /heapS_mapsto.
     iInv specN as (tp σ) ">[Hown %]" "Hclose".
     iDestruct (own_valid_2 with "Hown Hj")
-      as %[[?%tpool_singleton_included' _]%prod_included _]%auth_both_valid_discrete.
+      as %[[?%tpool_singleton_included' _]%prod_included _]
+          %auth_both_valid_discrete.
     iDestruct (own_valid_2 with "Hown Hl")
-      as %[[_ Hl%heap_singleton_included]%prod_included _]%auth_both_valid_discrete.
+      as %[[_ Hl%heap_singleton_included]%prod_included _]
+          %auth_both_valid_discrete.
     iMod (own_update_2 with "Hown Hj") as "[Hown Hj]".
     { by eapply auth_update, prod_local_update_1, singleton_local_update,
         (exclusive_local_update _ (Excl (fill K (#♭ true)))). }
@@ -376,6 +384,33 @@ Section cfg.
       by rewrite /to_heap lookup_fmap Hl. }
     iFrame "Hj Hl". iApply "Hclose". iNext.
     iExists (<[j:=fill K (#♭ true)]> tp), (<[l:=v2]>σ).
+    rewrite to_heap_insert to_tpool_insert'; last eauto. iFrame. iPureIntro.
+    eapply rtc_r, step_insert_no_fork; eauto. econstructor; eauto.
+  Qed.
+
+  Lemma step_faa E j K l m e2 k:
+    to_val e2 = Some (#nv k) → nclose specN ⊆ E →
+    spec_ctx ∗ j ⤇ fill K (FAA (Loc l) e2) ∗ l ↦ₛ (#nv m)
+    ={E}=∗ j ⤇ fill K (#n m) ∗ l ↦ₛ #nv (m + k).
+  Proof.
+    iIntros (??) "(#Hinv & Hj & Hl)"; subst. iDestruct "Hinv" as (ρ) "Hinv".
+    rewrite /spec_ctx /tpool_mapsto /heapS_mapsto.
+    iInv specN as (tp σ) ">[Hown %]" "Hclose".
+    iDestruct (own_valid_2 with "Hown Hj")
+      as %[[?%tpool_singleton_included' _]%prod_included _]
+          %auth_both_valid_discrete.
+    iDestruct (own_valid_2 with "Hown Hl")
+      as %[[_ Hl%heap_singleton_included]%prod_included _]
+          %auth_both_valid_discrete.
+    iMod (own_update_2 with "Hown Hj") as "[Hown Hj]".
+    { by eapply auth_update, prod_local_update_1, singleton_local_update,
+        (exclusive_local_update _ (Excl (fill K (#n m)))). }
+    iMod (own_update_2 with "Hown Hl") as "[Hown Hl]".
+    { eapply auth_update, prod_local_update_2, singleton_local_update,
+        (exclusive_local_update _ (1%Qp, to_agree (#nv (m + k)))); last done.
+      by rewrite /to_heap lookup_fmap Hl. }
+    iFrame "Hj Hl". iApply "Hclose". iNext.
+    iExists (<[j:=fill K (#n m)]> tp), (<[l:=#nv (m + k)]>σ).
     rewrite to_heap_insert to_tpool_insert'; last eauto. iFrame. iPureIntro.
     eapply rtc_r, step_insert_no_fork; eauto. econstructor; eauto.
   Qed.
@@ -409,9 +444,14 @@ Section cfg.
     spec_ctx ∗ j ⤇ fill K (TApp (TLam e)) ={E}=∗ j ⤇ fill K e.
   Proof. by intros ?; apply: do_step_pure. Qed.
 
-  Lemma step_Fold E j K e v :
+  Lemma step_fold E j K e v :
     to_val e = Some v → nclose specN ⊆ E →
     spec_ctx ∗ j ⤇ fill K (Unfold (Fold e)) ={E}=∗ j ⤇ fill K e.
+  Proof. by intros ?; apply: do_step_pure. Qed.
+
+  Lemma step_pack E j K e1 v e2 :
+    to_val e1 = Some v → nclose specN ⊆ E →
+    spec_ctx ∗ j ⤇ fill K (UnpackIn (Pack e1) e2) ={E}=∗ j ⤇ fill K e2.[e1/].
   Proof. by intros ?; apply: do_step_pure. Qed.
 
   Lemma step_fst E j K e1 v1 e2 v2 :
@@ -460,7 +500,8 @@ Section cfg.
     rewrite /spec_ctx /tpool_mapsto.
     iInv specN as (tp σ) ">[Hown %]" "Hclose".
     iDestruct (own_valid_2 with "Hown Hj")
-      as %[[?%tpool_singleton_included' _]%prod_included ?]%auth_both_valid_discrete.
+      as %[[?%tpool_singleton_included' _] %prod_included ?]
+          %auth_both_valid_discrete.
     assert (j < length tp) by eauto using lookup_lt_Some.
     iMod (own_update_2 with "Hown Hj") as "[Hown Hj]".
     { by eapply auth_update, prod_local_update_1,
