theories/logrel/stlc/fundamental.v
@@ -1,7 +1,12 @@
-From iris_examples.logrel.stlc Require Export logrel.
 From iris.proofmode Require Import tactics.
 From iris_examples.logrel.stlc Require Import rules.
 From iris.program_logic Require Import lifting.
+From iris_examples.logrel.stlc Require Export logrel.
+
+Definition log_typed `{irisG stlc_lang Σ}
+           (Γ : list type) (e : expr) (τ : type) : iProp Σ :=
+  □∀ vs, ⟦ Γ ⟧* vs -∗ ⟦ τ ⟧ₑ e.[env_subst vs].
+Notation "Γ ⊨ e : τ" := (log_typed Γ e τ) (at level 74, e, τ at next level).
 
 Section typed_interp.
   Context `{irisG stlc_lang Σ}.
@@ -11,11 +16,10 @@ Section typed_interp.
     iApply (wp_wand with "[-]"); [iApply Hp; trivial|]; cbn;
     iIntros (v) Hv.
 
-  Theorem fundamental Γ vs e τ :
-    Γ ⊢ₜ e : τ → ⟦ Γ ⟧* vs ⊢ ⟦ τ ⟧ₑ e.[env_subst vs].
+  Theorem fundamental Γ e τ : Γ ⊢ₜ e : τ → ⊢ Γ ⊨ e : τ.
   Proof.
-    intros Htyped; revert vs.
-    induction Htyped; iIntros (vs) "#Hctx /=".
+    intros Htyped.
+    induction Htyped; iIntros (vs) "!# #Hctx /=".
     - (* var *)
       iDestruct (interp_env_Some_l with "[]") as (v) "[#H1 #H2]"; eauto;
         iDestruct "H1" as %Heq. erewrite env_subst_lookup; eauto.
@@ -42,17 +46,17 @@ Section typed_interp.
       smart_wp_bind (CaseCtx _ _) v "# Hv" IHHtyped1; cbn.
       iDestruct "Hv" as "[Hv|Hv]"; iDestruct "Hv" as (w) "[% Hw]"; subst.
       + simpl. iApply wp_pure_step_later; auto. asimpl.
-        specialize (IHHtyped2 (w::vs)).
-        iNext. iApply (IHHtyped2). iApply interp_env_cons; by iSplit.
+        iApply (IHHtyped2 $! (w::vs)).
+        iNext. iApply interp_env_cons; by iSplit.
       + simpl. iApply wp_pure_step_later; auto. asimpl.
-        specialize (IHHtyped3 (w::vs)).
-        iNext. iApply (IHHtyped3). iApply interp_env_cons; by iSplit.
+        iApply (IHHtyped3 $! (w::vs)).
+        iNext. iApply interp_env_cons; by iSplit.
     - (* lam *)
       iDestruct (interp_env_length with "[]") as %Hlen; auto.
       iApply wp_value. simpl. iModIntro; iIntros (w) "#Hw".
       iApply wp_pure_step_later; auto.
       asimpl.
-      iNext; iApply (IHHtyped (w :: vs)). iApply interp_env_cons; by iSplit.
+      iNext; iApply (IHHtyped $! (w :: vs)). iApply interp_env_cons; by iSplit.
     - (* app *)
       smart_wp_bind (AppLCtx (e2.[env_subst vs])) v "#Hv" IHHtyped1.
       smart_wp_bind (AppRCtx v) w "#Hw" IHHtyped2.
